wip

Matroid/Equiv'.lean
@@ -5,16 +5,19 @@ namespace Matroid
 
 open Set LocalEquiv
 
-variable {α β α₁ α₂ α₃ : Type _} {M : Matroid α} {N : Matroid β}
+variable {α β α₁ α₂ α₃ : Type _} 
 
 structure Iso (M : Matroid α) (N : Matroid β) where
   (toLocalEquiv : LocalEquiv α β)
   (source_eq' : toLocalEquiv.source = M.E)
   (target_eq' : toLocalEquiv.target = N.E)
-  (setOf_base_eq : setOf N.Base = (image toLocalEquiv) '' (setOf M.Base))
+  (setOf_base_eq' : setOf N.Base = (image toLocalEquiv) '' (setOf M.Base))
 
 instance {M : Matroid α} {N : Matroid β} : CoeFun (Iso M N) (fun _ ↦ (α → β)) where
   coe e := (e.toLocalEquiv : α → β)  
+
+theorem Iso.setOf_base_eq (e : Iso M N) : setOf N.Base = (image e) '' (setOf M.Base) := 
+  e.setOf_base_eq'
 
 @[simp] lemma Iso.source_eq (e : Iso M N) : e.toLocalEquiv.source = M.E :=
   e.source_eq'
@@ -22,15 +25,23 @@ instance {M : Matroid α} {N : Matroid β} : CoeFun (Iso M N) (fun _ ↦ (α →
 @[simp] lemma Iso.target_eq (e : Iso M N) : e.toLocalEquiv.target = N.E :=
   e.target_eq'
 
-lemma Iso.injOn_ground (e : Iso M N) : InjOn e M.E := by
-  rw [←e.source_eq]; exact e.toLocalEquiv.injOn
+@[simp] lemma Iso.subset_source (e : Iso M N) (X : Set α) (hX : X ⊆ M.E := by aesop_mat) : 
+    X ⊆ e.toLocalEquiv.source := 
+  hX.trans_eq e.source_eq.symm
 
-theorem Iso.on_base (e : Iso M N) (hB : B ⊆ M.E) : M.Base B ↔ N.Base (e '' B) := by
-  change (_ ↔ _ ∈ setOf N.Base)
-  simp_rw [e.setOf_base_eq, mem_image, mem_setOf_eq]
-  refine' ⟨fun h ↦ ⟨B, h, rfl⟩, fun ⟨B', h, h'⟩ ↦ _⟩
-  rw [e.injOn_ground.image_eq_image_iff_of_subset h.subset_ground hB] at h'
-  rwa [←h']
+@[simp] lemma Iso.subset_target (e : Iso M N) (X : Set β) (hX : X ⊆ N.E := by aesop_mat) : 
+    X ⊆ e.toLocalEquiv.target := 
+  hX.trans_eq e.target_eq.symm  
+
+@[simp] lemma Iso.image_subset_target (e : Iso M N) (X : Set α) (hX : X ⊆ M.E := by aesop_mat) : 
+    e '' X ⊆ e.toLocalEquiv.target := by
+  rw [←image_source_eq_target]; exact image_subset _ (e.subset_source X)
+
+@[simp] lemma Iso.image_ground (e : Iso M N) : e '' M.E = N.E := by
+  rw [←e.source_eq, ←e.target_eq, image_source_eq_target] 
+
+lemma Iso.ground_subset_preimage_ground (e : Iso M N) : M.E ⊆ e ⁻¹' N.E := by 
+  rw [←e.source_eq, ←e.target_eq]; exact source_subset_preimage_target e.toLocalEquiv
 
 @[aesop unsafe 10% (rule_sets [Matroid])] 
 theorem Iso.image_subset_ground (e : Iso M N) (X : Set α) (hX : X ⊆ M.E := by aesop_mat) : 
@@ -38,18 +49,29 @@ theorem Iso.image_subset_ground (e : Iso M N) (X : Set α) (hX : X ⊆ M.E := by
   convert image_subset _ hX
   rw [←e.source_eq, image_source_eq_target, e.target_eq]
 
+lemma Iso.injOn_ground (e : Iso M N) : InjOn e M.E := by
+  rw [←e.source_eq]; exact e.toLocalEquiv.injOn
+
+theorem Iso.on_base_iff (e : Iso M N) (hB : B ⊆ M.E := by aesop_mat) :
+    M.Base B ↔ N.Base (e '' B) := by
+  change (_ ↔ _ ∈ setOf N.Base)
+  simp_rw [e.setOf_base_eq', mem_image, mem_setOf_eq]
+  refine' ⟨fun h ↦ ⟨B, h, rfl⟩, fun ⟨B', h, h'⟩ ↦ _⟩
+  rw [e.injOn_ground.image_eq_image_iff_of_subset h.subset_ground hB] at h'
+  rwa [←h']
+
 def Iso.refl (M : Matroid α) : Iso M M where
   toLocalEquiv := ofSet M.E 
   source_eq' := rfl 
   target_eq' := rfl
-  setOf_base_eq := by simp  
+  setOf_base_eq' := by simp  
 
 def Iso.symm (e : Iso M N) : Iso N M where
   toLocalEquiv := e.toLocalEquiv.symm
   source_eq' := by rw [symm_source, e.target_eq']
   target_eq' := by rw [symm_target, e.source_eq']
-  setOf_base_eq := by
-    { rw [e.setOf_base_eq]
+  setOf_base_eq' := by
+    { rw [e.setOf_base_eq']
       ext B
       simp only [mem_setOf_eq, mem_image, exists_exists_and_eq_and]
       refine' ⟨fun h ↦ ⟨B, h, _⟩, fun ⟨B', hB', h⟩ ↦ _⟩
@@ -68,12 +90,60 @@ def Iso.trans {M₁ : Matroid α₁} {M₂ : Matroid α₂} {M₃ : Matroid α�
   { rw [trans_target, e₁₂.target_eq', e₂₃.target_eq', inter_eq_left_iff_subset, 
       ←e₂₃.source_eq', ←e₂₃.target_eq']
     exact target_subset_preimage_source _ }
-  setOf_base_eq := by rw [e₂₃.setOf_base_eq, e₁₂.setOf_base_eq]; ext B; simp [image_image]
+  setOf_base_eq' := by rw [e₂₃.setOf_base_eq', e₁₂.setOf_base_eq']; ext B; simp [image_image]
 
 @[aesop unsafe 10% (rule_sets [Matroid])] 
 theorem Iso.image_symm_subset_ground (e : Iso M N) (X : Set β) (hX : X ⊆ N.E := by aesop_mat) : 
     e.symm '' X ⊆ M.E :=
   e.symm.image_subset_ground X hX 
+
+@[simp] theorem Iso.symm_apply (e : Iso M N) : e.symm.toLocalEquiv = e.toLocalEquiv.symm := rfl
+
+/-- Equal matroids are isomorphic -/
+def Iso.of_eq {M N : Matroid α} (h : M = N) : Iso M N where
+  toLocalEquiv := ofSet M.E
+  source_eq' := rfl
+  target_eq' := by simp [h]
+  setOf_base_eq' := by simp [h]
+  
+section transfer
+
+-- Some generic lemmas to carry a matroid `Set` property across an isomorphism 
+
+variable {PM : Set α → Prop} {PN : Set β → Prop} 
+
+/-- A matroid proposition transfers across an isomorphism-/
+theorem Iso.setOf_prop_eq (e : Iso M N) 
+    (hN : ∀ {Y}, PN Y → Y ⊆ N.E) (hMN : ∀ {X}, PM X → PN (e '' X)) 
+    (hNM : ∀ {Y}, PN Y → PM (e.symm '' Y)) : setOf PN = (image e) '' (setOf PM) := by 
+  refine' Set.ext (fun Y ↦ ⟨fun h ↦ _, _⟩)
+  · refine' ⟨e.symm '' Y, hNM h, _⟩  
+    rw [symm_apply, image_symm_image_of_subset_target _ ((hN h).trans_eq e.target_eq.symm)]
+  intro h; obtain ⟨X, hX, rfl⟩ := h
+  exact hMN hX
+
+theorem Iso.on_prop_symm (e : Iso M N) (on_prop : ∀ {Y}, PN Y → PM (e.symm '' Y)) (h : PN (e '' X)) 
+    (hX : X ⊆ M.E := by aesop_mat) : PM X := by
+  convert on_prop h; rw [symm_apply, symm_image_image_of_subset_source _ (e.subset_source X)]
+  
+theorem Iso.prop_subset_iff_subset (e : Iso M N) (hM : ∀ {X}, PM X → X ⊆ M.E) : 
+    ∀ ⦃X Y : Set α⦄, PM X → PM Y → (X ⊆ Y ↔ e '' X ⊆ e '' Y) := 
+  fun _ _ hX hY ↦ (e.injOn_ground.image_subset_image_iff_of_subset (hM hX) (hM hY)).symm
+  
+end transfer
+
+/-- A `LocalEquiv` that respects bases is an isomorphism. -/
+def Iso_of_forall_base (e : LocalEquiv α β) (hM : e.source = M.E) (hN : e.target = N.E) 
+    (on_base : ∀ B, M.Base B → N.Base (e '' B))
+    (on_base_symm : ∀ B, N.Base B → M.Base (e.symm '' B)) : Iso M N where
+  toLocalEquiv := e
+  source_eq' := hM
+  target_eq' := hN
+  setOf_base_eq' := by 
+  { refine' Set.ext (fun B ↦ ⟨fun (hB : N.Base B) ↦ ⟨_, on_base_symm B hB,_⟩,_⟩)
+    · rw [e.image_symm_image_of_subset_target (hB.subset_ground.trans_eq hN.symm)] 
+    rintro ⟨B, hB, rfl⟩
+    exact on_base B hB }
 
 /-- A `LocalEquiv` that respects independence is an isomorphism. -/
 def Iso_of_forall_indep (e : LocalEquiv α β) (hM : e.source = M.E) (hN : e.target = N.E) 
@@ -82,7 +152,7 @@ def Iso_of_forall_indep (e : LocalEquiv α β) (hM : e.source = M.E) (hN : e.tar
   toLocalEquiv := e
   source_eq' := hM
   target_eq' := hN
-  setOf_base_eq := by 
+  setOf_base_eq' := by 
   { have setOfIndep : setOf N.Indep = (Set.image e) '' (setOf M.Indep)
     · refine' subset_antisymm (fun I (hI : N.Indep I) ↦ ⟨_, on_indep_symm I hI, _⟩) _
       · rintro _ ⟨I, (hI : M.Indep I), rfl⟩; exact on_indep I hI
@@ -103,6 +173,9 @@ def Iso_of_forall_indep' (e : LocalEquiv α β) (hM : e.source = M.E) (hN : e.ta
       rwa [on_indep _ h', image_symm_image_of_subset_target _ 
         (by rw [hN]; exact hI.subset_ground)] })
 
+theorem Iso.on_base (e : Iso M N) (hB : M.Base B) : N.Base (e '' B) := by 
+  rwa [←e.on_base_iff]
+
 lemma Iso.on_indep (e : Iso M N) (hI : M.Indep I) : N.Indep (e '' I) := by
   change (_ ∈ (setOf N.Indep))
   rw [setOf_indep_eq, e.setOf_base_eq]
@@ -110,7 +183,19 @@ lemma Iso.on_indep (e : Iso M N) (hI : M.Indep I) : N.Indep (e '' I) := by
     image_subset_iff, exists_exists_and_eq_and]
   obtain ⟨B, hB, hIB⟩ := hI.exists_base_supset
   exact ⟨B, hB, hIB.trans (subset_preimage_image _ _)⟩ 
+
+theorem Iso.on_indep_symm (e : Iso M N) (h : N.Indep (e '' I)) (hI : I ⊆ M.E := by aesop_mat) : 
+    M.Indep I :=
+    e.on_prop_symm (e.symm.on_indep) h
   
+theorem Iso.setOf_indep_eq (e : Iso M N) : setOf N.Indep = (image e) '' (setOf M.Indep) :=
+  e.setOf_prop_eq Indep.subset_ground e.on_indep e.symm.on_indep
+  
+theorem Iso.on_base_symm (e : Iso M N) (h : N.Base (e '' B)) (hB : B ⊆ M.E := by aesop_mat) : 
+    M.Base B :=
+  e.on_prop_symm (e.symm.on_base) h
+
+/-- Restrictions of isomorphic matroids are isomorphic -/
 def Iso.restrict (e : Iso M N) (hR : R ⊆ M.E) : Iso (M | R) (N | (e '' R)) := 
   Iso_of_forall_indep (e.toLocalEquiv.restr R)
   (by simpa [restrict_ground_eq hR]) 
@@ -127,60 +212,57 @@ def Iso.restrict (e : Iso M N) (hR : R ⊆ M.E) : Iso (M | R) (N | (e '' R)) :=
     rw [image_eq_target_inter_inv_preimage _ (by rwa [e.source_eq])]
     apply inter_subset_right })
 
-
-/-- We write `M ≃i N` if there is an isomorphism from `M` to `N`. -/
-def IsIso (M : Matroid α) (N : Matroid β) : Prop := Nonempty (M.Iso N)
-
-infixl:65  " ≃i " => IsIso 
-
 /-- Restrict an isomorphism to a set not necessarily contained in the ground set.  -/
 def Iso.restrict' (e : Iso M N) (R : Set α) : Iso (M | (R ∩ M.E)) (N | (e '' (R ∩ M.E))) := 
-  Iso_of_forall_indep (e.toLocalEquiv.restr (R ∩ M.E)) 
-    (by simp)
-    (by { 
-      rw [restrict_ground_eq', restr_target, preimage_inter, ←e.source_eq, ←inter_assoc, inter_comm, 
-        ←inter_assoc, inter_eq_self_of_subset_right e.toLocalEquiv.target_subset_preimage_source, 
-        ←image_source_inter_eq', inter_comm R, eq_comm, inter_eq_left_iff_subset, ←e.target_eq, 
-        ←image_source_eq_target] 
-      exact image_subset _ (inter_subset_left _ _) } ) 
-    (by { 
-      simp only [restrict_indep_iff, subset_inter_iff, restr_coe, image_subset_iff, and_imp] 
-      exact fun I hI hIR hIE ↦ 
-        ⟨e.on_indep hI, (subset_inter hIR hIE).trans (subset_preimage_image _ _)⟩ })
+  (e.restrict (inter_subset_right R M.E))
+
+/-- The duals of isomorphic matroids are isomorphic -/
+def Iso.Dual (e : Iso M N) : Iso M﹡ N﹡ := 
+  Iso_of_forall_base e.toLocalEquiv 
+    (by simp) (by simp) 
     (by {
-      simp only [restrict_indep_iff, restr_coe_symm, image_subset_iff, and_imp]
-      refine' fun I hI hIss ↦ ⟨e.symm.on_indep hI,hIss.trans _⟩
-      rw [← e.source_eq, image_eq_target_inter_inv_preimage _ (inter_subset_right _ _)]
-      apply inter_subset_right })
+      simp_rw [dual_base_iff', image_subset_iff, and_imp]
+      refine fun B hB hBE ↦ ⟨?_, hBE.trans e.ground_subset_preimage_ground⟩
+      convert e.on_base hB
+      rw [e.injOn_ground.image_diff hBE, e.image_ground] } ) 
+    (by {
+      simp only [image_subset_iff, dual_base_iff', and_imp]
+      refine fun B hB hBE ↦ ⟨?_, hBE.trans e.symm.ground_subset_preimage_ground⟩
+      convert e.symm.on_base hB
+      rw [e.symm.injOn_ground.image_diff hBE, e.symm.image_ground, symm_apply] } )
 
--- theorem Iso.on_circuit (e : Iso M N) (h : M.Circuit C) : N.Circuit (e '' C) := by
---   rw [Circuit, setOf_dep_eq, setOf_indep_eq, e.setOf_base_eq]
---   rw [Circuit, setOf_dep_eq, setOf_indep_eq] at h
+theorem Iso.on_dep (e : Iso M N) (h : M.Dep D) : N.Dep (e '' D) := by 
+  rw [Dep, and_iff_left (e.image_subset_ground D)]; exact fun hI ↦ h.not_indep (e.on_indep_symm hI)
+
+theorem Iso.on_dep_symm (e : Iso M N) (h : N.Dep (e '' D)) (hD : D ⊆ M.E := by aesop_mat) : 
+    M.Dep D :=
+  e.on_prop_symm (e.symm.on_dep) h
+
+theorem Iso.setOf_dep_eq (e : Iso M N) : setOf N.Dep = (image e) '' setOf M.Dep :=
+  e.setOf_prop_eq Dep.subset_ground e.on_dep e.symm.on_dep
+
+theorem Iso.on_circuit (e : Iso M N) (h : M.Circuit C) : N.Circuit (e '' C) := by
+  rw [Circuit, e.setOf_dep_eq, minimals_image_of_rel_iff_rel (r := (· ⊆ ·))]
+  · exact mem_image_of_mem _ h
+  exact e.prop_subset_iff_subset Dep.subset_ground
   
+theorem Iso.on_circuit_symm (e : Iso M N) (h : N.Circuit (e '' C)) (hC : C ⊆ M.E := by aesop_mat) : 
+    M.Circuit C :=
+  e.on_prop_symm (e.symm.on_circuit) h
+
+theorem Iso.setOf_circuit_eq (e : Iso M N) : setOf N.Circuit = (image e) '' setOf M.Circuit :=
+  e.setOf_prop_eq (fun h ↦ h.1.subset_ground) e.on_circuit e.symm.on_circuit
+
+/-- We write `M ≃ N` if there is an isomorphism from `M` to `N`. -/
+def IsIso : Matroid α → Matroid β → Prop := fun M N ↦ Nonempty (M.Iso N)
+
+infixl:65  " ≃ " => IsIso 
+
+instance : IsEquiv (Matroid α) (fun (M N : Matroid α) ↦ M ≃ N) where
+  refl := fun M ↦ ⟨Iso.refl M⟩
+  trans := fun _ _ _ ⟨e⟩ ⟨e'⟩ ↦ ⟨e.trans e'⟩ 
+  symm := fun _ _ ⟨e⟩ ↦ ⟨e.symm⟩  
   
- 
-
-
-
--- def LocalEquiv.LocalEquivSet (i : LocalEquiv α β) : LocalEquiv (Set α) (Set β) where
---   toFun := image i.toFun
---   invFun := image i.invFun
---   source := Iic i.source
---   target := Iic i.target
---   map_source' := by 
---   { simp only [mem_Iic, le_eq_subset, image_subset_iff]
---     exact fun s hs a has ↦ i.map_source' (hs has) }
---   map_target' := by
---   { simp only [mem_Iic, le_eq_subset, image_subset_iff]
---     exact fun s hs a has ↦ i.map_target' (hs has) }
---   left_inv' := by
---   { simp only [mem_Iic, le_eq_subset, invFun_as_coe]
---     exact fun _ h ↦ symm_image_image_of_subset_source i h }
---   right_inv' := by
---   { simp only [mem_Iic, le_eq_subset, invFun_as_coe]
---     exact fun _ h ↦ image_symm_image_of_subset_target i h }
-
-
 
 
 
