Matroid/ForMathlib/Other.lean
@@ -11,3 +11,40 @@ lemma Set.InjOn.image_subset_image_iff_of_subset {f : α → β} (h : InjOn f s)
   refine' ⟨fun h' ↦ _, image_subset _⟩   
   rw [←h.preimage_image_inter h₁, ←h.preimage_image_inter h₂]
   exact inter_subset_inter_left _ (preimage_mono h')
+
+lemma Set.InjOn.image_diff' {f : α → β} (h : InjOn f s) : 
+    f '' (s \ t) = f '' s \ f '' (s ∩ t) := by
+  refine' Set.ext (fun y ↦ ⟨_,_⟩)
+  · rintro ⟨x, hx, rfl⟩
+    exact ⟨⟨x, hx.1, rfl⟩, fun h' ↦ hx.2 (h.mem_of_mem_image (inter_subset_left _ _) hx.1 h').2⟩ 
+  rintro ⟨⟨x, hx, rfl⟩,h'⟩
+  exact ⟨x, ⟨hx,fun hxt ↦ h' ⟨x, ⟨hx,hxt⟩, rfl⟩⟩, rfl⟩ 
+    
+lemma Set.InjOn.image_diff {f : α → β} (h : InjOn f s) (hst : t ⊆ s) : 
+    f '' (s \ t) = f '' s \ f '' t := by
+  rw [h.image_diff', inter_eq_self_of_subset_right hst]
+
+  
+
+
+
+-- def LocalEquiv.LocalEquivSet (i : LocalEquiv α β) : LocalEquiv (Set α) (Set β) where
+--   toFun := image i.toFun
+--   invFun := image i.invFun
+--   source := Iic i.source
+--   target := Iic i.target
+--   map_source' := by 
+--   { simp only [mem_Iic, le_eq_subset, image_subset_iff]
+--     exact fun s hs a has ↦ i.map_source' (hs has) }
+--   map_target' := by
+--   { simp only [mem_Iic, le_eq_subset, image_subset_iff]
+--     exact fun s hs a has ↦ i.map_target' (hs has) }
+--   left_inv' := by
+--   { simp only [mem_Iic, le_eq_subset, invFun_as_coe]
+--     exact fun _ h ↦ symm_image_image_of_subset_source i h }
+--   right_inv' := by
+--   { simp only [mem_Iic, le_eq_subset, invFun_as_coe]
+--     exact fun _ h ↦ image_symm_image_of_subset_target i h }
+
+
+  
